src/coq/Theory/InstrLemmas.v
@@ -32,11 +32,11 @@ Open Scope itree_scope.
 (** Helper lemmas that should probably be moved *)
 
 (* TODO: Move this *)
-Lemma interp_cfg_to_L3_concretize_or_pick_concrete :
+Lemma interp_cfg3_concretize_or_pick_concrete :
   forall (uv : uvalue) (dv : dvalue) P g ρ m,
     is_concrete uv ->
     uvalue_to_dvalue uv = inr dv ->
-    interp_cfg_to_L3 (concretize_or_pick uv P) g ρ m ≈ Ret (m, (ρ, (g, dv))).
+    interp_cfg3 (concretize_or_pick uv P) g ρ m ≈ Ret (m, (ρ, (g, dv))).
 Proof.
   intros uv dv P g ρ m CONC CONV.
   unfold concretize_or_pick.
@@ -44,7 +44,7 @@ Proof.
   cbn.
   unfold lift_err.
   rewrite CONV.
-  rewrite interp_cfg_to_L3_ret.
+  rewrite interp_cfg3_ret.
   reflexivity.
 Qed.
 
@@ -124,25 +124,25 @@ Proof with reflexivity.
 Qed.
 
 (* TODO: Move this *)
-Lemma interp_cfg_to_L3_concretize_or_pick_concrete_exists :
+Lemma interp_cfg3_concretize_or_pick_concrete_exists :
   forall (uv : uvalue) P g ρ m,
     is_concrete uv ->
-    exists dv, uvalue_to_dvalue uv = inr dv /\ interp_cfg_to_L3 (concretize_or_pick uv P) g ρ m ≈ Ret (m, (ρ, (g, dv))).
+    exists dv, uvalue_to_dvalue uv = inr dv /\ interp_cfg3 (concretize_or_pick uv P) g ρ m ≈ Ret (m, (ρ, (g, dv))).
 Proof.
   intros uv P g ρ m CONC.
   pose proof is_concrete_uvalue_to_dvalue uv CONC as (dv & CONV).
   exists dv.
   split; auto.
-  apply interp_cfg_to_L3_concretize_or_pick_concrete; auto.
+  apply interp_cfg3_concretize_or_pick_concrete; auto.
 Qed.
 
 (* TODO: Move this *)
-Lemma interp_cfg_to_L3_pick :
+Lemma interp_cfg3_pick :
   forall uv P g ρ m,
-    interp_cfg_to_L3 (trigger (pick uv P)) g ρ m ≈ ITree.bind (trigger (pick uv P)) (fun dv => Ret (m, (ρ, (g, dv)))).
+    interp_cfg3 (trigger (pick uv P)) g ρ m ≈ ITree.bind (trigger (pick uv P)) (fun dv => Ret (m, (ρ, (g, dv)))).
 Proof.
   intros uv P g ρ m.
-  unfold interp_cfg_to_L3.
+  unfold interp_cfg3.
 
   rewrite interp_intrinsics_trigger.
   cbn.
@@ -176,15 +176,15 @@ Proof.
 Qed.
 
 (* TODO; Move this *)
-Lemma interp_cfg_to_L3_concretize_or_pick_not_concrete :
+Lemma interp_cfg3_concretize_or_pick_not_concrete :
   forall (uv : uvalue) (dv : dvalue) P g ρ m,
     is_concrete uv = false ->
-    interp_cfg_to_L3 (concretize_or_pick uv P) g ρ m ≈ ITree.bind (trigger (pick uv P)) (fun dv => Ret (m, (ρ, (g, dv)))).
+    interp_cfg3 (concretize_or_pick uv P) g ρ m ≈ ITree.bind (trigger (pick uv P)) (fun dv => Ret (m, (ρ, (g, dv)))).
 Proof.
   intros uv dv P g ρ m NCONC.
   unfold concretize_or_pick.
   rewrite NCONC.
-  rewrite interp_cfg_to_L3_pick.
+  rewrite interp_cfg3_pick.
   reflexivity.
 Qed.
 
@@ -192,70 +192,70 @@ Qed.
 
 Lemma denote_instr_load :
   forall (i : raw_id) volatile τ τp ptr align g ρ ρ' m a uv,
-    interp_cfg_to_L3 (translate exp_E_to_instr_E (denote_exp (Some τp) ptr)) g ρ m ≈ Ret (m, (ρ', (g, UVALUE_Addr a))) ->
+    interp_cfg3 (translate exp_E_to_instr_E (denote_exp (Some τp) ptr)) g ρ m ≈ Ret (m, (ρ', (g, UVALUE_Addr a))) ->
     read m a τ = inr uv ->
-    interp_cfg_to_L3 (denote_instr (IId i, INSTR_Load volatile τ (τp, ptr) align)) g ρ m ≈ Ret (m, (Maps.add i uv ρ', (g, tt))).
+    interp_cfg3 (denote_instr (IId i, INSTR_Load volatile τ (τp, ptr) align)) g ρ m ≈ Ret (m, (Maps.add i uv ρ', (g, tt))).
 Proof.
   intros i volatile τ τp ptr align g ρ ρ' m a uv EXP READ.
   cbn.
-  rewrite interp_cfg_to_L3_bind.
+  rewrite interp_cfg3_bind.
   rewrite EXP.
   rewrite bind_ret_l.
   cbn.
   rewrite bind_ret_l.
-  rewrite interp_cfg_to_L3_bind.
-  rewrite interp_cfg_to_L3_Load; eauto.
+  rewrite interp_cfg3_bind.
+  rewrite interp_cfg3_Load; eauto.
 
   rewrite bind_ret_l.
-  rewrite interp_cfg_to_L3_LW.
+  rewrite interp_cfg3_LW.
   cbn.
   reflexivity.
 Qed.
 
 Lemma denote_instr_store :
   forall (i : int) volatile τv val τp ptr align uv dv a g ρ ρ' ρ'' m m',
-    interp_cfg_to_L3 (translate exp_E_to_instr_E (denote_exp (Some τv) val)) g ρ m ≈ Ret (m, (ρ', (g, uv))) ->
-    interp_cfg_to_L3 (translate exp_E_to_instr_E (denote_exp (Some τp) ptr)) g ρ' m ≈ Ret (m, (ρ'', (g, UVALUE_Addr a))) ->
+    interp_cfg3 (translate exp_E_to_instr_E (denote_exp (Some τv) val)) g ρ m ≈ Ret (m, (ρ', (g, uv))) ->
+    interp_cfg3 (translate exp_E_to_instr_E (denote_exp (Some τp) ptr)) g ρ' m ≈ Ret (m, (ρ'', (g, UVALUE_Addr a))) ->
     uvalue_to_dvalue uv = inr dv ->
     write m a dv = inr m' ->
-    interp_cfg_to_L3 (denote_instr (IVoid i, INSTR_Store volatile (τv, val) (τp, ptr) align)) g ρ m ≈ Ret (m', (ρ'', (g, tt))).
+    interp_cfg3 (denote_instr (IVoid i, INSTR_Store volatile (τv, val) (τp, ptr) align)) g ρ m ≈ Ret (m', (ρ'', (g, tt))).
 Proof.
   intros i volatile τv val τp ptr align uv dv a g ρ ρ' ρ'' m m' EXP PTR CONV_UV WRITE.
   cbn.
-  rewrite interp_cfg_to_L3_bind.
+  rewrite interp_cfg3_bind.
   rewrite EXP.
   rewrite bind_ret_l.
-  rewrite interp_cfg_to_L3_bind.
+  rewrite interp_cfg3_bind.
 
   pose proof (uvalue_to_dvalue_is_concrete _ _ CONV_UV) as CONC_UV.
-  eapply interp_cfg_to_L3_concretize_or_pick_concrete_exists in CONC_UV as (dv' & CONV_UV' & CONC_UV).
+  eapply interp_cfg3_concretize_or_pick_concrete_exists in CONC_UV as (dv' & CONV_UV' & CONC_UV).
   rewrite CONV_UV' in CONV_UV.
   injection CONV_UV; intros; subst.
   rewrite CONC_UV.
 
   rewrite bind_ret_l.
-  rewrite interp_cfg_to_L3_bind.
+  rewrite interp_cfg3_bind.
   rewrite PTR.
   rewrite bind_ret_l.
 
-  rewrite interp_cfg_to_L3_bind.
+  rewrite interp_cfg3_bind.
   cbn.
-  rewrite interp_cfg_to_L3_ret.
+  rewrite interp_cfg3_ret.
   rewrite bind_ret_l.
 
-  rewrite interp_cfg_to_L3_store; cbn; eauto.
+  rewrite interp_cfg3_store; cbn; eauto.
   reflexivity.
 Qed.
 
 Lemma denote_instr_store_exists :
   forall (i : int) volatile τv val τp ptr align uv dv a g ρ ρ' ρ'' m,
-    interp_cfg_to_L3 (translate exp_E_to_instr_E (denote_exp (Some τv) val)) g ρ m ≈ Ret (m, (ρ', (g, uv))) ->
-    interp_cfg_to_L3 (translate exp_E_to_instr_E (denote_exp (Some τp) ptr)) g ρ' m ≈ Ret (m, (ρ'', (g, UVALUE_Addr a))) ->
+    interp_cfg3 (translate exp_E_to_instr_E (denote_exp (Some τv) val)) g ρ m ≈ Ret (m, (ρ', (g, uv))) ->
+    interp_cfg3 (translate exp_E_to_instr_E (denote_exp (Some τp) ptr)) g ρ' m ≈ Ret (m, (ρ'', (g, UVALUE_Addr a))) ->
     uvalue_to_dvalue uv = inr dv ->
     dvalue_has_dtyp dv τv ->
     dtyp_fits m a τv ->
     exists m',
-      write m a dv = inr m' /\ interp_cfg_to_L3 (denote_instr (IVoid i, INSTR_Store volatile (τv, val) (τp, ptr) align)) g ρ m ≈ Ret (m', (ρ'', (g, tt))).
+      write m a dv = inr m' /\ interp_cfg3 (denote_instr (IVoid i, INSTR_Store volatile (τv, val) (τp, ptr) align)) g ρ m ≈ Ret (m', (ρ'', (g, tt))).
 Proof.
   intros i volatile τv val τp ptr align uv dv a g ρ ρ' ρ'' m EXP PTR CONV_UV TYP FITS.
   apply write_succeeds with (v:=dv) in FITS as [m2 WRITE]; auto.
@@ -268,40 +268,40 @@ Lemma denote_instr_alloca_exists :
     non_void τ ->
     exists m' a,
       allocate m τ = inr (m', a) /\
-      interp_cfg_to_L3 (denote_instr (IId i, INSTR_Alloca τ nb align)) g ρ m ≈ Ret (m', (Maps.add i (UVALUE_Addr a) ρ, (g, tt))).
+      interp_cfg3 (denote_instr (IId i, INSTR_Alloca τ nb align)) g ρ m ≈ Ret (m', (Maps.add i (UVALUE_Addr a) ρ, (g, tt))).
 Proof.
   intros m τ g ρ i align nb NV.
 
-  pose proof interp_cfg_to_L3_alloca m τ g ρ NV as (m' & a & ALLOC & TRIGGER).
+  pose proof interp_cfg3_alloca m τ g ρ NV as (m' & a & ALLOC & TRIGGER).
   exists m'. exists a. split; auto.
 
-  cbn. rewrite interp_cfg_to_L3_bind.
+  cbn. rewrite interp_cfg3_bind.
   rewrite TRIGGER; cbn.
   rewrite bind_ret_l.
-  rewrite interp_cfg_to_L3_LW. cbn.
+  rewrite interp_cfg3_LW. cbn.
   reflexivity.
 Qed.
 
 Lemma denote_instr_comment :
   forall i str g ρ m,
-    interp_cfg_to_L3 (denote_instr (i, INSTR_Comment str)) g ρ m ≈ Ret (m, (ρ, (g, tt))).
+    interp_cfg3 (denote_instr (i, INSTR_Comment str)) g ρ m ≈ Ret (m, (ρ, (g, tt))).
 Proof.
   intros i str g ρ m.
-  destruct i; cbn; rewrite interp_cfg_to_L3_ret; reflexivity.
+  destruct i; cbn; rewrite interp_cfg3_ret; reflexivity.
 Qed.
 
 Lemma denote_instr_op :
   forall (i : raw_id) (op : exp dtyp) uv g ρ ρ' m,
-    interp_cfg_to_L3 (translate exp_E_to_instr_E (denote_exp None op)) g ρ m ≈ Ret (m, (ρ', (g, uv))) ->
-    interp_cfg_to_L3 (denote_instr (IId i, INSTR_Op op)) g ρ m ≈ Ret (m, (Maps.add i uv ρ', (g, tt))).
+    interp_cfg3 (translate exp_E_to_instr_E (denote_exp None op)) g ρ m ≈ Ret (m, (ρ', (g, uv))) ->
+    interp_cfg3 (denote_instr (IId i, INSTR_Op op)) g ρ m ≈ Ret (m, (Maps.add i uv ρ', (g, tt))).
 Proof.
   intros i op uv g ρ ρ' m OP.
   cbn.
   unfold denote_op.
-  rewrite interp_cfg_to_L3_bind.
+  rewrite interp_cfg3_bind.
 
   rewrite OP. rewrite bind_ret_l.
-  rewrite interp_cfg_to_L3_LW.
+  rewrite interp_cfg3_LW.
   reflexivity.
 Qed.
 
@@ -315,11 +315,11 @@ Qed.
 
 Lemma denote_instr_gep_array :
   forall i size τ e_ix ix ptr a val g ρ m,
-    interp_cfg_to_L3 (translate exp_E_to_instr_E (denote_exp (Some DTYPE_Pointer) ptr)) g ρ m
+    interp_cfg3 (translate exp_E_to_instr_E (denote_exp (Some DTYPE_Pointer) ptr)) g ρ m
     ≈
     Ret (m, (ρ, (g, UVALUE_Addr a)))
     ->
-    interp_cfg_to_L3 (translate exp_E_to_instr_E (denote_exp (Some (DTYPE_I 64)) e_ix)) g ρ m
+    interp_cfg3 (translate exp_E_to_instr_E (denote_exp (Some (DTYPE_I 64)) e_ix)) g ρ m
     ≈
     Ret (m, (ρ, (g, UVALUE_I64 (repr (Z.of_nat ix)))))
     ->
@@ -327,19 +327,19 @@ Lemma denote_instr_gep_array :
     ->
     exists ptr_res,
       read m ptr_res τ = inr val /\
-      interp_cfg_to_L3 (denote_instr (IId i, INSTR_Op (OP_GetElementPtr (DTYPE_Array size τ) (DTYPE_Pointer, ptr) [(DTYPE_I 64, EXP_Integer 0%Z); (DTYPE_I 64, e_ix)]))) g ρ m
+      interp_cfg3 (denote_instr (IId i, INSTR_Op (OP_GetElementPtr (DTYPE_Array size τ) (DTYPE_Pointer, ptr) [(DTYPE_I 64, EXP_Integer 0%Z); (DTYPE_I 64, e_ix)]))) g ρ m
       ≈
       Ret (m, (Maps.add i (UVALUE_Addr ptr_res) ρ, (g, tt))).
 Proof.
   intros i size τ e_ix ix ptr a val g ρ m PTR IX GET.
 
-  pose proof interp_cfg_to_L3_GEP_array τ a size g ρ m val ix GET as (ptr_res & EQ & READ).
+  pose proof interp_cfg3_GEP_array τ a size g ρ m val ix GET as (ptr_res & EQ & READ).
   exists ptr_res. split; auto.
 
   cbn.
   rewrite translate_bind.
   rewrite bind_bind.
-  rewrite interp_cfg_to_L3_bind.
+  rewrite interp_cfg3_bind.
 
   rewrite PTR.
   rewrite bind_ret_l.
@@ -352,14 +352,14 @@ Proof.
   repeat rewrite translate_bind.
   repeat rewrite bind_bind.
 
-  rewrite interp_cfg_to_L3_bind.
+  rewrite interp_cfg3_bind.
   rewrite IX.
   rewrite bind_ret_l.
 
-  rewrite interp_cfg_to_L3_bind.
+  rewrite interp_cfg3_bind.
   rewrite bind_ret_l.
   rewrite translate_ret.
-  rewrite interp_cfg_to_L3_ret.
+  rewrite interp_cfg3_ret.
   rewrite bind_ret_l.
   rewrite translate_ret.
   rewrite bind_ret_l.
@@ -369,28 +369,28 @@ Proof.
   rewrite bind_bind.
 
   rewrite translate_trigger.
-  rewrite interp_cfg_to_L3_bind_trigger.
+  rewrite interp_cfg3_bind_trigger.
   rewrite exp_E_to_instr_E_subevent.
 
   rewrite EQ.
 
   rewrite bind_ret_l.
-  rewrite interp_cfg_to_L3_bind.
+  rewrite interp_cfg3_bind.
   cbn.
   rewrite translate_ret.
-  rewrite interp_cfg_to_L3_ret.
+  rewrite interp_cfg3_ret.
   rewrite bind_ret_l.
-  rewrite interp_cfg_to_L3_LW.
+  rewrite interp_cfg3_LW.
   reflexivity.
 Qed.
 
 Lemma denote_instr_gep_array' :
   forall i size τ e_ix ix ptr a val g ρ m,
-    interp_cfg_to_L3 (translate exp_E_to_instr_E (denote_exp (Some DTYPE_Pointer) ptr)) g ρ m
+    interp_cfg3 (translate exp_E_to_instr_E (denote_exp (Some DTYPE_Pointer) ptr)) g ρ m
     ≈
     Ret (m, (ρ, (g, UVALUE_Addr a)))
     ->
-    interp_cfg_to_L3 (translate exp_E_to_instr_E (denote_exp (Some (DTYPE_I 64)) e_ix)) g ρ m
+    interp_cfg3 (translate exp_E_to_instr_E (denote_exp (Some (DTYPE_I 64)) e_ix)) g ρ m
     ≈
     Ret (m, (ρ, (g, UVALUE_I64 (repr (Z.of_nat ix)))))
     ->
@@ -399,13 +399,13 @@ Lemma denote_instr_gep_array' :
     exists ptr_res,
       read m ptr_res τ = inr val /\
       handle_gep_addr (DTYPE_Array size τ) a [DVALUE_I64 (repr 0); DVALUE_I64 (repr (Z.of_nat ix))] = inr ptr_res /\
-      interp_cfg_to_L3 (denote_instr (IId i, INSTR_Op (OP_GetElementPtr (DTYPE_Array size τ) (DTYPE_Pointer, ptr) [(DTYPE_I 64, EXP_Integer 0%Z); (DTYPE_I 64, e_ix)]))) g ρ m
+      interp_cfg3 (denote_instr (IId i, INSTR_Op (OP_GetElementPtr (DTYPE_Array size τ) (DTYPE_Pointer, ptr) [(DTYPE_I 64, EXP_Integer 0%Z); (DTYPE_I 64, e_ix)]))) g ρ m
       ≈
       Ret (m, (Maps.add i (UVALUE_Addr ptr_res) ρ, (g, tt))).
 Proof.
   intros i size τ e_ix ix ptr a val g ρ m PTR IX GET.
 
-  pose proof interp_cfg_to_L3_GEP_array' τ a size g ρ m val ix GET as (ptr_res & EQ & GEP & READ).
+  pose proof interp_cfg3_GEP_array' τ a size g ρ m val ix GET as (ptr_res & EQ & GEP & READ).
   exists ptr_res.
   split; auto.
   split; auto.
@@ -413,7 +413,7 @@ Proof.
   cbn.
   rewrite translate_bind.
   rewrite bind_bind.
-  rewrite interp_cfg_to_L3_bind.
+  rewrite interp_cfg3_bind.
 
   rewrite PTR.
   rewrite bind_ret_l.
@@ -426,14 +426,14 @@ Proof.
   repeat rewrite translate_bind.
   repeat rewrite bind_bind.
 
-  rewrite interp_cfg_to_L3_bind.
+  rewrite interp_cfg3_bind.
   rewrite IX.
   rewrite bind_ret_l.
 
-  rewrite interp_cfg_to_L3_bind.
+  rewrite interp_cfg3_bind.
   rewrite bind_ret_l.
   rewrite translate_ret.
-  rewrite interp_cfg_to_L3_ret.
+  rewrite interp_cfg3_ret.
   rewrite bind_ret_l.
   rewrite translate_ret.
   rewrite bind_ret_l.
@@ -443,18 +443,18 @@ Proof.
   rewrite bind_bind.
 
   rewrite translate_trigger.
-  rewrite interp_cfg_to_L3_bind_trigger.
+  rewrite interp_cfg3_bind_trigger.
   rewrite exp_E_to_instr_E_subevent.
 
   rewrite EQ.
 
   rewrite bind_ret_l.
-  rewrite interp_cfg_to_L3_bind.
+  rewrite interp_cfg3_bind.
   cbn.
   rewrite translate_ret.
-  rewrite interp_cfg_to_L3_ret.
+  rewrite interp_cfg3_ret.
   rewrite bind_ret_l.
-  rewrite interp_cfg_to_L3_LW.
+  rewrite interp_cfg3_LW.
   reflexivity.
 Qed.
 
@@ -462,27 +462,27 @@ Qed.
 
 Lemma denote_instr_gep_array_no_read_addr :
   forall i size τ e_ix ix ptr a g ρ m ptr_res,
-    interp_cfg_to_L3 (translate exp_E_to_instr_E (denote_exp (Some DTYPE_Pointer) ptr)) g ρ m
+    interp_cfg3 (translate exp_E_to_instr_E (denote_exp (Some DTYPE_Pointer) ptr)) g ρ m
     ≈
     Ret (m, (ρ, (g, UVALUE_Addr a)))
     ->
-    interp_cfg_to_L3 (translate exp_E_to_instr_E (denote_exp (Some (DTYPE_I 64)) e_ix)) g ρ m
+    interp_cfg3 (translate exp_E_to_instr_E (denote_exp (Some (DTYPE_I 64)) e_ix)) g ρ m
     ≈
     Ret (m, (ρ, (g, UVALUE_I64 (repr (Z.of_nat ix)))))
     ->
     dtyp_fits m a (DTYPE_Array size τ) ->
     handle_gep_addr (DTYPE_Array size τ) a [DVALUE_I64 (Int64.repr 0); DVALUE_I64 (Int64.repr (Z.of_nat ix))] = inr ptr_res ->
-    interp_cfg_to_L3 (denote_instr (IId i, INSTR_Op (OP_GetElementPtr (DTYPE_Array size τ) (DTYPE_Pointer, ptr) [(DTYPE_I 64, EXP_Integer 0%Z); (DTYPE_I 64, e_ix)]))) g ρ m
+    interp_cfg3 (denote_instr (IId i, INSTR_Op (OP_GetElementPtr (DTYPE_Array size τ) (DTYPE_Pointer, ptr) [(DTYPE_I 64, EXP_Integer 0%Z); (DTYPE_I 64, e_ix)]))) g ρ m
       ≈
       Ret (m, (Maps.add i (UVALUE_Addr ptr_res) ρ, (g, tt))).
 Proof.
   intros * PTR IX FITS HGEP.
-  pose proof @interp_cfg_to_L3_GEP_array_no_read_addr τ a size g ρ m ix ptr_res FITS.
+  pose proof @interp_cfg3_GEP_array_no_read_addr τ a size g ρ m ix ptr_res FITS.
 
   cbn.
   rewrite translate_bind.
   rewrite bind_bind.
-  rewrite interp_cfg_to_L3_bind.
+  rewrite interp_cfg3_bind.
 
   rewrite PTR.
   rewrite bind_ret_l.
@@ -495,14 +495,14 @@ Proof.
   repeat rewrite translate_bind.
   repeat rewrite bind_bind.
 
-  rewrite interp_cfg_to_L3_bind.
+  rewrite interp_cfg3_bind.
   rewrite IX.
   rewrite bind_ret_l.
 
-  rewrite interp_cfg_to_L3_bind.
+  rewrite interp_cfg3_bind.
   rewrite bind_ret_l.
   rewrite translate_ret.
-  rewrite interp_cfg_to_L3_ret.
+  rewrite interp_cfg3_ret.
   rewrite bind_ret_l.
   rewrite translate_ret.
   rewrite bind_ret_l.
@@ -512,48 +512,48 @@ Proof.
   rewrite bind_bind.
 
   rewrite translate_trigger.
-  rewrite interp_cfg_to_L3_bind_trigger.
+  rewrite interp_cfg3_bind_trigger.
   rewrite exp_E_to_instr_E_subevent.
 
   rewrite H; auto.
 
   rewrite bind_ret_l.
-  rewrite interp_cfg_to_L3_bind.
+  rewrite interp_cfg3_bind.
   cbn.
   rewrite translate_ret.
-  rewrite interp_cfg_to_L3_ret.
+  rewrite interp_cfg3_ret.
   rewrite bind_ret_l.
-  rewrite interp_cfg_to_L3_LW.
+  rewrite interp_cfg3_LW.
   reflexivity.
 Qed.
 
 Lemma denote_instr_gep_array_no_read :
   forall i size τ e_ix ix ptr a g ρ m,
-    interp_cfg_to_L3 (translate exp_E_to_instr_E (denote_exp (Some DTYPE_Pointer) ptr)) g ρ m
+    interp_cfg3 (translate exp_E_to_instr_E (denote_exp (Some DTYPE_Pointer) ptr)) g ρ m
     ≈
     Ret (m, (ρ, (g, UVALUE_Addr a)))
     ->
-    interp_cfg_to_L3 (translate exp_E_to_instr_E (denote_exp (Some (DTYPE_I 64)) e_ix)) g ρ m
+    interp_cfg3 (translate exp_E_to_instr_E (denote_exp (Some (DTYPE_I 64)) e_ix)) g ρ m
     ≈
     Ret (m, (ρ, (g, UVALUE_I64 (repr (Z.of_nat ix)))))
     ->
     dtyp_fits m a (DTYPE_Array size τ) ->
     exists ptr_res,
       handle_gep_addr (DTYPE_Array size τ) a [DVALUE_I64 (repr 0); DVALUE_I64 (repr (Z.of_nat ix))] = inr ptr_res /\
-      interp_cfg_to_L3 (denote_instr (IId i, INSTR_Op (OP_GetElementPtr (DTYPE_Array size τ) (DTYPE_Pointer, ptr) [(DTYPE_I 64, EXP_Integer 0%Z); (DTYPE_I 64, e_ix)]))) g ρ m
+      interp_cfg3 (denote_instr (IId i, INSTR_Op (OP_GetElementPtr (DTYPE_Array size τ) (DTYPE_Pointer, ptr) [(DTYPE_I 64, EXP_Integer 0%Z); (DTYPE_I 64, e_ix)]))) g ρ m
       ≈
       Ret (m, (Maps.add i (UVALUE_Addr ptr_res) ρ, (g, tt))).
 Proof.
   intros i size τ e_ix ix ptr a g ρ m PTR IX FITS.
 
-  pose proof interp_cfg_to_L3_GEP_array_no_read τ a size g ρ m ix FITS as (ptr_res & EQ & GEP).
+  pose proof interp_cfg3_GEP_array_no_read τ a size g ρ m ix FITS as (ptr_res & EQ & GEP).
   exists ptr_res.
   split; auto.
 
   cbn.
   rewrite translate_bind.
   rewrite bind_bind.
-  rewrite interp_cfg_to_L3_bind.
+  rewrite interp_cfg3_bind.
 
   rewrite PTR.
   rewrite bind_ret_l.
@@ -566,14 +566,14 @@ Proof.
   repeat rewrite translate_bind.
   repeat rewrite bind_bind.
 
-  rewrite interp_cfg_to_L3_bind.
+  rewrite interp_cfg3_bind.
   rewrite IX.
   rewrite bind_ret_l.
 
-  rewrite interp_cfg_to_L3_bind.
+  rewrite interp_cfg3_bind.
   rewrite bind_ret_l.
   rewrite translate_ret.
-  rewrite interp_cfg_to_L3_ret.
+  rewrite interp_cfg3_ret.
   rewrite bind_ret_l.
   rewrite translate_ret.
   rewrite bind_ret_l.
@@ -583,18 +583,18 @@ Proof.
   rewrite bind_bind.
 
   rewrite translate_trigger.
-  rewrite interp_cfg_to_L3_bind_trigger.
+  rewrite interp_cfg3_bind_trigger.
   rewrite exp_E_to_instr_E_subevent.
 
   rewrite EQ.
 
   rewrite bind_ret_l.
-  rewrite interp_cfg_to_L3_bind.
+  rewrite interp_cfg3_bind.
   cbn.
   rewrite translate_ret.
-  rewrite interp_cfg_to_L3_ret.
+  rewrite interp_cfg3_ret.
   rewrite bind_ret_l.
-  rewrite interp_cfg_to_L3_LW.
+  rewrite interp_cfg3_LW.
   reflexivity.
 Qed.
 
@@ -604,17 +604,17 @@ Lemma denote_instr_intrinsic :
     ->
     assoc in_n (defs_assoc) = Some sem_f
     ->
-    interp_cfg_to_L3 (map_monad (fun '(t, op) => translate exp_E_to_instr_E (denote_exp (Some t) op)) args) g ρ m
+    interp_cfg3 (map_monad (fun '(t, op) => translate exp_E_to_instr_E (denote_exp (Some t) op)) args) g ρ m
     ≈
     Ret (m, (ρ, (g, arg_vs))) 
     ->
-    interp_cfg_to_L3 (map_monad (fun uv : uvalue => pickUnique uv) arg_vs) g ρ m
+    interp_cfg3 (map_monad (fun uv : uvalue => pickUnique uv) arg_vs) g ρ m
     ≈
     Ret (m, (ρ, (g, conc_args)))
     ->
     sem_f conc_args = inr res
     ->
-    (interp_cfg_to_L3
+    (interp_cfg3
        (denote_instr
           (IId i,
            INSTR_Call (τ, EXP_Ident (ID_Global (Name fn))) args)) g ρ m)
@@ -624,77 +624,77 @@ Proof.
   intros * INTRINSIC ASSOC  MAP CONCARGS RES.
 
   unfold denote_instr.
-  setoid_rewrite interp_cfg_to_L3_bind.
+  setoid_rewrite interp_cfg3_bind.
   rewrite MAP.
   setoid_rewrite bind_ret_l.
   rewrite INTRINSIC.
   setoid_rewrite bind_bind.
-  rewrite interp_cfg_to_L3_bind.
+  rewrite interp_cfg3_bind.
   rewrite CONCARGS.
   rewrite bind_ret_l.
 
   cbn; unfold ITree.map.
   rewrite bind_bind.
-  rewrite interp_cfg_to_L3_bind.
-  rewrite interp_cfg_to_L3_intrinsic; eauto.
+  rewrite interp_cfg3_bind.
+  rewrite interp_cfg3_intrinsic; eauto.
 
   repeat (cbn; rewrite bind_ret_l).
-  rewrite interp_cfg_to_L3_LW.
+  rewrite interp_cfg3_LW.
   cbn.
   reflexivity.
 Qed.
 
 Lemma denote_term_br_l :
   forall (e : exp dtyp) b1 b2 g ρ ρ' m,
-    interp_cfg_to_L3 (translate exp_E_to_instr_E (denote_exp (Some (DTYPE_I 1)) e)) g ρ m
+    interp_cfg3 (translate exp_E_to_instr_E (denote_exp (Some (DTYPE_I 1)) e)) g ρ m
     ≈
     Ret (m, (ρ', (g, UVALUE_I1 one)))
     ->
-    interp_cfg_to_L3 (translate exp_E_to_instr_E (denote_terminator (TERM_Br (DTYPE_I 1%N, e) b1 b2))) g ρ m
+    interp_cfg3 (translate exp_E_to_instr_E (denote_terminator (TERM_Br (DTYPE_I 1%N, e) b1 b2))) g ρ m
     ≈
     Ret (m, (ρ', (g, inl b1))).
 Proof.
   intros * EXP.
   simpl.
-  rewrite translate_bind, interp_cfg_to_L3_bind.
+  rewrite translate_bind, interp_cfg3_bind.
   rewrite EXP, bind_ret_l.
   cbn.
   rewrite bind_ret_l.
   cbn.
-  rewrite translate_ret,interp_cfg_to_L3_ret.
+  rewrite translate_ret,interp_cfg3_ret.
   reflexivity.
 Qed.
 
 Lemma denote_term_br_r :
   forall (e : exp dtyp) b1 b2 g ρ ρ' m,
-    interp_cfg_to_L3 (translate exp_E_to_instr_E (denote_exp (Some (DTYPE_I 1)) e)) g ρ m
+    interp_cfg3 (translate exp_E_to_instr_E (denote_exp (Some (DTYPE_I 1)) e)) g ρ m
     ≈
     Ret (m, (ρ', (g, UVALUE_I1 zero)))
     ->
-    interp_cfg_to_L3 (translate exp_E_to_instr_E (denote_terminator (TERM_Br (DTYPE_I 1%N, e) b1 b2))) g ρ m
+    interp_cfg3 (translate exp_E_to_instr_E (denote_terminator (TERM_Br (DTYPE_I 1%N, e) b1 b2))) g ρ m
     ≈
     Ret (m, (ρ', (g, inl b2))).
 Proof.
   intros * EXP.
   simpl.
-  rewrite translate_bind, interp_cfg_to_L3_bind.
+  rewrite translate_bind, interp_cfg3_bind.
   rewrite EXP, bind_ret_l.
   cbn.
   rewrite bind_ret_l.
   cbn.
-  rewrite translate_ret,interp_cfg_to_L3_ret.
+  rewrite translate_ret,interp_cfg3_ret.
   reflexivity.
 Qed.
 
 Lemma denote_term_br_1 :
   forall b g ρ m,
-    interp_cfg_to_L3 (translate exp_E_to_instr_E (denote_terminator (TERM_Br_1 b))) g ρ m
+    interp_cfg3 (translate exp_E_to_instr_E (denote_terminator (TERM_Br_1 b))) g ρ m
     ≈
     Ret (m, (ρ, (g, inl b))).
 Proof.
   intros b g ρ m.
   cbn.
-  rewrite translate_ret,interp_cfg_to_L3_ret.
+  rewrite translate_ret,interp_cfg3_ret.
   reflexivity.
 Qed.
 
@@ -724,36 +724,36 @@ Qed.
 
 (*
 
-interp_cfg_to_L3_intrinsic:
+interp_cfg3_intrinsic:
   forall (defs : Intrinsics.intrinsic_definitions) (m : memory_stack) (τ : dtyp)
     (g : global_env) (l : local_env) (fn : String.string) (args : list dvalue)
     (df : Intrinsics.semantic_function) (res : dvalue),
   assoc Strings.String.string_dec fn (defs_assoc) = Some df ->
   df args = inr res ->
-  Monad.eqm (interp_cfg_to_L3 (trigger (Intrinsic τ fn args)) g l m) (ret (m, (l, (g, res))))
+  Monad.eqm (interp_cfg3 (trigger (Intrinsic τ fn args)) g l m) (ret (m, (l, (g, res))))
 
 *)
 
 (* Lemma denote_instr_call : *)
 (*   forall i τf f args uf uvs g ρ ρ' m t, *)
 (*     map_monad (fun '(t, op) => translate exp_E_to_instr_E (denote_exp (Some t) op)) args ≈ Ret uvs -> *)
-(*     interp_cfg_to_L3 (translate exp_E_to_instr_E (denote_exp None f)) g ρ m ≈ Ret (m, (ρ', (g, uf))) -> *)
+(*     interp_cfg3 (translate exp_E_to_instr_E (denote_exp None f)) g ρ m ≈ Ret (m, (ρ', (g, uf))) -> *)
 (*     intrinsic_exp f = None -> *)
-(*     interp_cfg_to_L3 (denote_instr (IId i, INSTR_Call (τf, f) args)) g ρ m ≈ t. (* interp_cfg_to_L3 (ITree.bind (trigger (LLVMEvents.Call τf uf uvs)) (fun x => trigger (LocalWrite i x)) g ρ' m). *) *)
+(*     interp_cfg3 (denote_instr (IId i, INSTR_Call (τf, f) args)) g ρ m ≈ t. (* interp_cfg3 (ITree.bind (trigger (LLVMEvents.Call τf uf uvs)) (fun x => trigger (LocalWrite i x)) g ρ' m). *) *)
 (* Proof. *)
 (*   intros i τf f args uf uvs g ρ ρ' m t MAP FEXP INT. *)
 (*   cbn. *)
 (*   rewrite MAP. rewrite bind_ret_l. *)
 (*   rewrite INT. rewrite bind_bind. *)
 
-(*   rewrite interp_cfg_to_L3_bind. *)
+(*   rewrite interp_cfg3_bind. *)
 (*   rewrite FEXP. rewrite bind_ret_l. *)
 
-(*   rewrite interp_cfg_to_L3_bind. *)
-(*   rewrite interp_cfg_to_L3_LW. *)
+(*   rewrite interp_cfg3_bind. *)
+(*   rewrite interp_cfg3_LW. *)
 (*   rewrite <- bind_trigger. *)
 
-(*   interp_cfg_to_L3 *)
+(*   interp_cfg3 *)
 (*     (ITree.bind (trigger (LLVMEvents.Call τf uf uvs)) *)
 (*        (fun returned_value : uvalue => trigger (LocalWrite i returned_value))) g ρ' m ≈ t *)
 
